stdlib/vec/extra_specs.v
@@ -3,11 +3,11 @@ Section Vec_inv_t_ne.
 
   Global Instance Vec_inv_t_contr {rt1 T_rt A_rt} (T : type rt1 → type T_rt) (A : type A_rt) :
     TypeNonExpansive T →
-    TypeContractive (λ ty, Vec_inv_t (T ty) A).
+    TypeContractive (λ ty, Vec_inv_t T_rt A_rt <TY> (T ty) <TY> A <INST!>).
   Proof.
   Admitted.
   Global Instance Vec_inv_t_ne {rt1 T_rt A_rt} (T : type rt1 → type T_rt) (A : type A_rt) :
     TypeNonExpansive T →
-    TypeNonExpansive (λ ty, Vec_inv_t (T ty) A).
+    TypeNonExpansive (λ ty, Vec_inv_t T_rt A_rt <TY> (T ty) <TY> A <INST!>).
   Proof. Admitted.
-End Vec_inv_t_ne. 
+End Vec_inv_t_ne.
